SSA/Projects/InstCombine/AliveHandwrittenLargeExamples.lean
@@ -4,6 +4,7 @@ import SSA.Projects.InstCombine.LLVM.PrettyEDSL
 import SSA.Projects.InstCombine.Tactic
 import SSA.Projects.InstCombine.TacticAuto
 import SSA.Projects.InstCombine.ComWrappers
+import SSA.Projects.InstCombine.LLVM.Semantics
 import Mathlib.Tactic
 
 open BitVec
@@ -134,6 +135,7 @@ def alive_simplifyMulDivRem805 (w : Nat) :
       rw [LLVM.sdiv?_denom_zero_eq_none]
       apply Refinement.none_left
     case neg =>
+      simp
       rw [BitVec.ult_toNat]
       rw [BitVec.toNat_ofNat]
       cases w'
@@ -227,6 +229,7 @@ def alive_simplifyMulDivRem805' (w : Nat) :
   unfold MulDivRem805_lhs MulDivRem805_rhs
   simp only [simp_llvm_wrap]
   simp_alive_ssa
+  simp only [LLVM.add_reduce]
   simp_alive_undef
   simp_alive_case_bash
   simp only [ofInt_ofNat, add_eq, LLVM.icmp?_ult_eq]
